check-footprints.bash
@@ -293,6 +293,10 @@ ROBINSON_PlusPlus.Meta.ChainNegPrf.dico_FTT|propext,Classical.choice,Quot.sound
 ROBINSON_PlusPlus.Meta.ChainNegPrf.decodes_leibniz|propext,Classical.choice,Quot.sound
 ROBINSON_PlusPlus.Meta.ChainNegPrf.decodeForm_termCode|propext,Classical.choice,Quot.sound
 ROBINSON_PlusPlus.Meta.ChainNegPrf.cierra_tag0|propext,Classical.choice,Quot.sound,FOL.MetaRules.ex_elim,FOL.MetaRules.imp_intro,FOL.MetaRules.or_elim,FOL.MetaRules.raa,ROBINSON_PlusPlus.Full.ax_induction_prim,ROBINSON_PlusPlus.Full.ax_list_induction
+ROBINSON_PlusPlus.Meta.CodeDistinct.formCode_ne_notFC|propext,Classical.choice,Quot.sound,FOL.MetaRules.ex_elim,FOL.MetaRules.imp_intro,FOL.MetaRules.or_elim,FOL.MetaRules.raa,ROBINSON_PlusPlus.Full.ax_induction_prim
+ROBINSON_PlusPlus.Meta.ChainNegPrf.cierra_FF|propext,Classical.choice,Quot.sound,FOL.MetaRules.ex_elim,FOL.MetaRules.imp_intro,FOL.MetaRules.or_elim,FOL.MetaRules.raa,ROBINSON_PlusPlus.Full.ax_induction_prim,ROBINSON_PlusPlus.Full.ax_list_induction
+ROBINSON_PlusPlus.Meta.ChainNegPrf.cierra_c1|propext,Classical.choice,Quot.sound,FOL.MetaRules.ex_elim,FOL.MetaRules.imp_intro,FOL.MetaRules.or_elim,FOL.MetaRules.raa,ROBINSON_PlusPlus.Full.ax_induction_prim,ROBINSON_PlusPlus.Full.ax_list_induction
+ROBINSON_PlusPlus.Meta.ChainNegPrf.cierra_qconf|propext,Classical.choice,Quot.sound,FOL.MetaRules.ex_elim,FOL.MetaRules.imp_intro,FOL.MetaRules.or_elim,FOL.MetaRules.raa,ROBINSON_PlusPlus.Full.ax_induction_prim,ROBINSON_PlusPlus.Full.ax_list_induction
 ROBINSON_PlusPlus.Meta.ChainNegPrf.deuda_inNeg|Classical.choice,FOL.MetaRules.ex_elim,FOL.MetaRules.imp_intro,FOL.MetaRules.or_elim,FOL.MetaRules.raa,Quot.sound,ROBINSON_PlusPlus.Full.ax_induction_prim,ROBINSON_PlusPlus.Full.ax_list_induction,propext
 ROBINSON_PlusPlus.Meta.CodeWitnessPrf.SinWTs.prf_isTermCodeE1_of_In|Classical.choice,Quot.sound,propext
 ROBINSON_PlusPlus.Meta.D3BodyPrf.hA_lineWFDotAt|Classical.choice,Quot.sound,propext
